Attempt to implement Equal and start proof
The test for equality in bvp to word is substantially more complicated
given Word64s, since now heap data must be compared as opposed to just
pointers. The header word for byte arrays has been tweaked (an
additional fixed 1 bit) so they can be distinguished from Word64s. I
don't know why every header word needs the bottom 2 bits set, though, so
maybe there is a better scheme.

Currently cheated:
  - that if the two pointers are equal, then what is pointed to is
    equal. this appears to come down to injectivity of get_addr and is
    not as trivial as it seems it should be.
  - the meat of the Word64 comparison, i.e., that the loaded words are
    in memory and that the comparisons implement equality of the
    represented word64s.

compiler/backend/bvp_to_wordScript.sml
@@ -161,9 +161,29 @@ val assign_def = Define `
                             Const 1w])],l))
     | Label n => (LocValue (adjust_var dest) (2 * n + bvl_to_bvi$num_stubs) 0,l)
     | Equal => (case args of
-               | [v1;v2] => (If Equal (adjust_var v1) (Reg (adjust_var v2))
-                              (Assign (adjust_var dest) TRUE_CONST)
-                              (Assign (adjust_var dest) FALSE_CONST),l)
+               | [v1;v2] =>
+                 let retf = Assign (adjust_var dest) FALSE_CONST in
+                 let rett = Assign (adjust_var dest) TRUE_CONST in
+                 (If Equal (adjust_var v1) (Reg (adjust_var v2)) rett
+                    (If Test (adjust_var v1) (Imm 1w) retf
+                       (Seq (Assign 1 (Load (real_addr c (adjust_var v1))))
+                          (If Test 1 (Imm 4w) retf
+                             (If Test 1 (Imm 16w)
+                               (let a1 = real_addr c (adjust_var v1) in
+                                let a2 = real_addr c (adjust_var v2) in
+                                list_Seq [
+                                  Assign 1 (Load (Op Add [a1; Const bytes_in_word]));
+                                  Assign 3 (Load (Op Add [a2; Const bytes_in_word]));
+                                  If Equal 1 (Reg 3)
+                                    (if dimindex (:'a) = 32 then rett
+                                     else
+                                       list_Seq [
+                                         Assign 1 (Load (Op Add [a1; Const (bytes_in_word <<1)]));
+                                         Assign 3 (Load (Op Add [a2; Const (bytes_in_word <<1)]));
+                                         If Equal 1 (Reg 3) rett retf])
+                                    retf])
+                               retf))))
+                 ,l)
                 | _ => (Skip,l))
     | Less => (case args of
                | [v1;v2] => (If Less (adjust_var v1) (Reg (adjust_var v2))
